<?xml version='1.0' encoding='ISO-8859-1'?>

<!--
  This document uses XML entities as abbreviations for URIs.
  -->

<!DOCTYPE uridef[
  <!ENTITY rdf "http://www.w3.org/1999/02/22-rdf-syntax-ns">
  <!--Added for shadow list vocab-->
  <!ENTITY shadow-rdf "http://localhost:8888/owl_s/1.1/generic/ObjectList.owl">
  <!ENTITY rdfs "http://www.w3.org/2000/01/rdf-schema">
  <!ENTITY owl "http://www.w3.org/2002/07/owl">
  <!ENTITY xsd "http://www.w3.org/2001/XMLSchema">
  <!ENTITY service "http://localhost:8888/owl_s/1.1/Service.owl">
  <!ENTITY process "http://localhost:8888/owl_s/1.1/Process.owl">
  <!ENTITY DEFAULT "http://localhost:8888/owl_s/1.1/Grounding.owl">
]>


<rdf:RDF
  xmlns:rdf=	 "&rdf;#"
  xmlns:shadow-rdf = "&shadow-rdf;#"
  xmlns:rdfs=	 "&rdfs;#"
  xmlns:owl =    "&owl;#"
  xmlns:service= "&service;#"
  xmlns:process= "&process;#"
  xmlns=	 "&DEFAULT;#"
  xml:base=      "&DEFAULT;">

<owl:Ontology rdf:about="">
  <owl:versionInfo>
    $Id: Grounding.owl 2269 2009-08-19 15:21:09Z thorsten $
  </owl:versionInfo>
  <rdfs:comment>
    Upper-level OWL ontology for Groundings that employ WSDL.
    Part of the OWL-S ontology; see http://www.daml.org/services/.

    This version is intended for use with WSDL 1.1.  The OWL-S
    Coalition plans to produce a future version for use with WSDL 2.0,
    when it has been finalized (or nearly so).

    Note that other approaches to grounding may be accommodated
    within the OWL-S framework.  This is the only approach produced
    to date by the OWL-S Coalition.

    For notes on version history, see 
        http://localhost:8888/owl_s/1.1/status.html.    
  </rdfs:comment>
  <owl:imports>
	<owl:Ontology rdf:about="&process;"/>
  </owl:imports>
</owl:Ontology>


<!--######################################################
    WsdlGrounding
    ######################################################-->

<owl:Class rdf:ID="WsdlGrounding">
  <rdfs:comment>
    A WsdlGrounding is just a collection of WsdlAtomicProcessGrounding
    instances, one for each atomic process in the process model.
  </rdfs:comment>
  <rdfs:subClassOf rdf:resource="&service;#ServiceGrounding"/>
</owl:Class>

<owl:ObjectProperty rdf:ID="hasAtomicProcessGrounding">
  <rdfs:domain rdf:resource="#WsdlGrounding"/>
  <rdfs:range rdf:resource="#WsdlAtomicProcessGrounding"/>
</owl:ObjectProperty>


<!--######################################################
    WsdlAtomicProcessGrounding
    ######################################################-->

<owl:Class rdf:ID="WsdlAtomicProcessGrounding">
  <rdfs:comment>
    A class that relates elements of a OWL-S atomic process to a
    WSDL specification.
  </rdfs:comment>
  <rdfs:comment>
    Each instance of WsdlAtomicProcessGrounding must have exactly one
    value for owlsProcess and exactly one for wsdlOperation, which sets up
    a one-to-one correspondence between an atomic process and a WSDL
    operation.

    In addition, for each message part of the relevant WSDL input message,
    there must be exactly one value of wsdlInput.  For each output of the
    atomic process, there must be exactly one value of wsdlOutput. These
    property instances show the correspondences between OWL-S
    inputs/outputs and WSDL message parts.  In addition, single values are
    recommended (but not required) for wsdlInputMessage and
    wsdlOutputMessage.

    Note that the value of wsdlOperation may or may not uniquely identify
    a particular WSDL port with which to interact.  If there are multiple
    such ports offering the specified operation, an OWL-S enactment engine
    is free to choose any of these ports.  If it is desired to further
    constrain the choice of ports, a WsdlAtomicProcessGrounding may do so
    by specifying any number of values for wsdlService and/or wsdlPort.
  </rdfs:comment>
  <rdfs:subClassOf>
    <owl:Restriction>
      <owl:onProperty rdf:resource="#owlsProcess"/>
     <owl:cardinality rdf:datatype="&xsd;#nonNegativeInteger">1</owl:cardinality>
    </owl:Restriction>
  </rdfs:subClassOf>
</owl:Class>

<!-- owlsProcess -->

<owl:ObjectProperty rdf:ID="owlsProcess">
  <rdfs:comment>
    The atomic process to which this grounding applies.
  </rdfs:comment>
  <rdfs:domain rdf:resource="#WsdlAtomicProcessGrounding"/>
  <rdfs:range rdf:resource="&process;#AtomicProcess"/>
</owl:ObjectProperty>
<owl:FunctionalProperty rdf:about="#owlsProcess"/>

<!-- wsdlOperation -->
  
<owl:ObjectProperty rdf:ID="wsdlOperation">
  <rdfs:comment>
    A WSDL operation to which the atomic process
    (referenced by owlsProcess) corresponds.
  </rdfs:comment>
  <rdfs:domain rdf:resource="#WsdlAtomicProcessGrounding"/>
  <rdfs:range rdf:resource="#WsdlOperationRef"/>
</owl:ObjectProperty>

<!-- wsdlService -->

<owl:DatatypeProperty rdf:ID="wsdlService">
  <rdfs:comment>
    A URI for a WSDL Service that provides the operation to which 
    this atomic process is grounded.
  </rdfs:comment>
  <rdfs:domain rdf:resource="#WsdlAtomicProcessGrounding"/>
  <rdfs:range rdf:resource="&xsd;#anyURI"/>
</owl:DatatypeProperty>

<!-- wsdlPort -->

<owl:DatatypeProperty rdf:ID="wsdlPort">
  <rdfs:comment>
    A URI for a WSDL Port that provides the operation to which 
    this atomic process is grounded.
  </rdfs:comment>
  <rdfs:domain rdf:resource="#WsdlAtomicProcessGrounding"/>
  <rdfs:range rdf:resource="&xsd;#anyURI"/>
</owl:DatatypeProperty> 

<!-- wsdlInputMessage -->

<owl:DatatypeProperty rdf:ID="wsdlInputMessage">
  <rdfs:comment>
    A URI for the WSDL input message element corresponding
    to the inputs of the atomic process.
  </rdfs:comment>
  <rdf:type rdf:resource="&owl;#FunctionalProperty"/>
  <rdfs:domain rdf:resource="#WsdlAtomicProcessGrounding"/>
  <rdfs:range rdf:resource="&xsd;#anyURI"/>
</owl:DatatypeProperty>

<!-- wsdlInput -->

<owl:ObjectProperty rdf:ID="wsdlInput">
  <rdfs:comment>
    There should be one instance of this property for each
    message part of the WSDL input message.
  </rdfs:comment>
  <rdfs:domain rdf:resource="#WsdlAtomicProcessGrounding"/>
  <rdfs:range rdf:resource="#WsdlInputMessageMap"/>
</owl:ObjectProperty>

<!-- wsdlOutputMessage -->

<owl:DatatypeProperty rdf:ID="wsdlOutputMessage">
  <rdfs:comment>
    A URI for the WSDL message element corresponding
    to the outputs of the atomic process.
  </rdfs:comment>
  <rdf:type rdf:resource="&owl;#FunctionalProperty"/>
  <rdfs:domain rdf:resource="#WsdlAtomicProcessGrounding"/>
  <rdfs:range rdf:resource="&xsd;#anyURI"/>
</owl:DatatypeProperty>

<!-- wsdlOutput -->
<owl:ObjectProperty rdf:ID="wsdlOutput">
  <rdfs:comment>
    There should be one instance of this property for each
    output of the atomic process.
  </rdfs:comment>
  <rdfs:domain rdf:resource="#WsdlAtomicProcessGrounding"/>
  <rdfs:range rdf:resource="#WsdlOutputMessageMap"/>
</owl:ObjectProperty>

<!-- wsdlVersion -->

<owl:DatatypeProperty rdf:ID="wsdlVersion">
  <rdfs:comment>
    A URI indicating the version of WSDL being used.
  </rdfs:comment>
  <rdf:type rdf:resource="&owl;#FunctionalProperty"/>
  <rdfs:domain rdf:resource="#WsdlAtomicProcessGrounding"/>
  <rdfs:range rdf:resource="&xsd;#anyURI"/>
</owl:DatatypeProperty>

<!-- wsdlDocument -->

<owl:DatatypeProperty rdf:ID="wsdlDocument">
  <rdfs:comment>
    A URI indicating a WSDL document to
    which this grounding refers.  This isn't
    essential; primarily for convenience as documentation.
  </rdfs:comment>
  <rdfs:domain rdf:resource="#WsdlAtomicProcessGrounding"/>
  <rdfs:range rdf:resource="&xsd;#anyURI"/>
</owl:DatatypeProperty>


<!--######################################################
    WsdlOperationRef
    ######################################################-->

<owl:Class rdf:ID="WsdlOperationRef">
 <rdfs:comment>
    This class provides a unique specification of a WSDL operation.
    WSDL 1.1, on which this version of the grounding is based, does 
    not have a way to uniquely identify an operation with a single URI.  
    Uniqueness is achieved using a pair (portType, operation).
  </rdfs:comment>
</owl:Class>

<owl:DatatypeProperty rdf:ID="portType">
  <rdfs:domain rdf:resource="#WsdlOperationRef" />
  <rdfs:range rdf:resource="&xsd;#anyURI" />
</owl:DatatypeProperty>

<owl:DatatypeProperty rdf:ID="operation">
  <rdfs:domain rdf:resource="#WsdlOperationRef"/>
  <rdfs:range rdf:resource="&xsd;#anyURI"/>
</owl:DatatypeProperty>

<owl:Class rdf:about="#WsdlOperationRef">
  <rdfs:comment>
    Restricting the cardinality of portType to one
  </rdfs:comment>
  <rdfs:subClassOf>
    <owl:Restriction>
      <owl:onProperty rdf:resource="#portType"/>     
      <owl:cardinality rdf:datatype="&xsd;#nonNegativeInteger">1</owl:cardinality>
    </owl:Restriction>
  </rdfs:subClassOf>
</owl:Class>

<owl:Class rdf:about="#WsdlOperationRef">
  <rdfs:comment>
    Restricting the cardinality of operation to one
  </rdfs:comment>
  <rdfs:subClassOf>
    <owl:Restriction>
      <owl:onProperty rdf:resource="#operation"/>     
      <owl:cardinality rdf:datatype="&xsd;#nonNegativeInteger">1</owl:cardinality>
    </owl:Restriction>
  </rdfs:subClassOf>
</owl:Class>


<!--######################################################
    WsdlMessageMap, WsdlInputMessageMap, WsdlOutputMessageMap

    To get the gist of these classes, read the comments for
    WsdlInputMessageMap and WsdlOutputMessageMap.
    ######################################################-->

<owl:Class rdf:ID="WsdlMessageMap">
  <rdfs:comment>
    Superclass for WsdlInputMessageMap and WsdlOutputMessageMap.
  </rdfs:comment>
</owl:Class>

<!-- owlsParameter -->

<owl:ObjectProperty rdf:ID="owlsParameter">
  <rdfs:comment>
    An input or output property of an atomic process.
  </rdfs:comment>
  <rdfs:domain rdf:resource="#WsdlMessageMap"/>
  <rdfs:range rdf:resource="&process;#Parameter"/>
</owl:ObjectProperty>

<!-- wsdlMessagePart -->

<owl:DatatypeProperty rdf:ID="wsdlMessagePart">
  <rdfs:comment>
    A URI for a WSDL message part element.
  </rdfs:comment>
  <rdfs:domain rdf:resource="#WsdlMessageMap"/>
  <rdfs:range rdf:resource="&xsd;#anyURI"/>
</owl:DatatypeProperty>

<owl:DatatypeProperty rdf:ID="xsltTransformation">
  <rdfs:comment>
    XSLT Tranformation to transform OWL-S parameters (inputs and outputs) 
    to and from WSDL messages.  This property exists mainly for declaring
    a cardinality restriction, and should not be instantiated
    directly.  Instantiate xsltTransformationString or xsltTransformationURI.
    (Ranges are specified with the sub properties.)
  </rdfs:comment>
  <rdfs:domain rdf:resource="#WsdlMessageMap"/>
</owl:DatatypeProperty>

<owl:DatatypeProperty rdf:ID="xsltTransformationString">
  <rdfs:subPropertyOf rdf:resource="#xsltTransformation"/>
  <rdfs:comment>
    A string giving an XSLT Tranformation.
  </rdfs:comment>
  <rdfs:range rdf:resource="&xsd;#string"/>
</owl:DatatypeProperty>

<owl:DatatypeProperty rdf:ID="xsltTransformationURI">
  <rdfs:subPropertyOf rdf:resource="#xsltTransformation"/>
  <rdfs:comment>
    A URI for an XSLT Tranformation.
  </rdfs:comment>
  <rdfs:range rdf:resource="&xsd;#anyURI"/>
</owl:DatatypeProperty>

<owl:Class rdf:ID="WsdlInputMessageMap">
  <rdfs:subClassOf rdf:resource="#WsdlMessageMap"/>
  <rdfs:comment>
    A class that shows how to derive a WSDL message part from 
    (one or more) inputs of an atomic process.
    A WsdlInputMessageMap must have 1 wsdlMessagePart, and 
    EITHER 1 owlsParameter or 1 xsltTransformation.  (The
    cardinality restrictions don't capture the disjunction.)
    If there is a direct correspondence between a particular
    OWL-S input and the wsdlMessagePart, use owlsParameter
    to show that.  Otherwise, use xsltTransformation to give
    a transformation from the OWL-S input(s) to the
    wsdlMessagePart.
  </rdfs:comment>
  <rdfs:subClassOf>
    <owl:Restriction>
      <owl:onProperty rdf:resource="#wsdlMessagePart"/>
      <owl:cardinality rdf:datatype="&xsd;#nonNegativeInteger">1</owl:cardinality>
    </owl:Restriction>
  </rdfs:subClassOf>
  <rdfs:subClassOf>
    <owl:Restriction>
      <owl:onProperty rdf:resource="#owlsParameter"/>     
      <owl:maxCardinality rdf:datatype="&xsd;#nonNegativeInteger">1</owl:maxCardinality>
    </owl:Restriction>
  </rdfs:subClassOf>
  <rdfs:subClassOf>
    <owl:Restriction>
      <owl:onProperty rdf:resource="#xsltTransformation"/>
      <owl:maxCardinality rdf:datatype="&xsd;#nonNegativeInteger">1</owl:maxCardinality>
    </owl:Restriction>
  </rdfs:subClassOf>
</owl:Class>

<owl:Class rdf:ID="WsdlOutputMessageMap">
  <rdfs:subClassOf rdf:resource="#WsdlMessageMap"/>
  <rdfs:comment>
    A class that shows how to derive an atomic process output from 
    the input message parts of a WSDL operation.
    A WsdlOutputMessageMap must have 1 owlsParameter, and 
    EITHER 1 wsdlMessagePart or 1 xsltTransformation.  (The
    cardinality restrictions don't capture the disjunction.)
    If there is a direct correspondence between a particular
    WSDL message part and the OWL-S output, use wsdlMessagePart
    to show that.  Otherwise, use xsltTransformation to give
    a transformation from the message parts to the OWL-S output.
  </rdfs:comment>
  <rdfs:subClassOf>
    <owl:Restriction>
      <owl:onProperty rdf:resource="#owlsParameter"/>
      <owl:cardinality rdf:datatype="&xsd;#nonNegativeInteger">1</owl:cardinality>
    </owl:Restriction>
  </rdfs:subClassOf>
  <rdfs:subClassOf>
    <owl:Restriction>
      <owl:onProperty rdf:resource="#wsdlMessagePart"/>
      <owl:maxCardinality rdf:datatype="&xsd;#nonNegativeInteger">1</owl:maxCardinality>
    </owl:Restriction>
  </rdfs:subClassOf>
  <rdfs:subClassOf>
    <owl:Restriction>
      <owl:onProperty rdf:resource="#xsltTransformation"/>
      <owl:maxCardinality rdf:datatype="&xsd;#nonNegativeInteger">1</owl:maxCardinality>
    </owl:Restriction>
  </rdfs:subClassOf>
</owl:Class>

<!--######################################################
  Everything below here is deprecated.
  ######################################################-->

<owl:ObjectProperty rdf:ID="wsdlInputMessageParts">
  <rdfs:comment>
    Deprecated as of DAML-S 0.9.
  </rdfs:comment>
  <owl:equivalentProperty rdf:resource="#wsdlInputs"/>
</owl:ObjectProperty>
<owl:FunctionalProperty rdf:about="#wsdlInputMessageParts"/>

<owl:ObjectProperty rdf:ID="wsdlOutputMessageParts">
  <rdfs:comment>
    Deprecated as of DAML-S 0.9; wsdlOutputs should now be used.
  </rdfs:comment>
  <owl:equivalentProperty rdf:resource="#wsdlOutputs"/>
</owl:ObjectProperty>
<owl:FunctionalProperty rdf:about="#wsdlOutputMessageParts"/>

<owl:DatatypeProperty rdf:ID="wsdlReference">
  <rdfs:comment>
    Deprecated as of DAML-S 0.9; wsdlVersion should now be used.
  </rdfs:comment>
  <rdfs:domain rdf:resource="#WsdlAtomicProcessGrounding"/>
  <rdfs:range rdf:resource="&xsd;#anyURI"/>
  <rdf:type rdf:resource="&owl;#FunctionalProperty"/>
  <owl:equivalentProperty rdf:resource="#wsdlVersion"/>
</owl:DatatypeProperty>

<!-- otherReference -->

<owl:DatatypeProperty rdf:ID="otherReference">
  <rdfs:comment>
    A URI indicating a relevant standards document (other than that
    for WSDL).
    Deprecated as of DAML-S 0.9; no longer recommended or supported.
  </rdfs:comment>
  <rdfs:domain rdf:resource="#WsdlAtomicProcessGrounding"/>
  <rdfs:range rdf:resource="&xsd;#anyURI"/>
</owl:DatatypeProperty>

<!-- damlsParameter -->

<owl:ObjectProperty rdf:ID="damlsParameter">
  <rdfs:comment>
    Deprecated as of OWL-S 1.0.  owlsParameter should be used.
  </rdfs:comment>
  <owl:equivalentProperty rdf:resource="#owlsParameter"/>
</owl:ObjectProperty>

<!-- wsdlInputs -->

<owl:ObjectProperty rdf:ID="wsdlInputs">
  <rdfs:comment>
    Deprecated as of OWL-S 1.0.  wsdlInput should be used.
  </rdfs:comment>
  <rdfs:comment>
    A list of WsdlMessageMap instances, one for each
    message part of the WSDL input message.
  </rdfs:comment>
  <rdfs:domain rdf:resource="#WsdlAtomicProcessGrounding"/>
  <rdfs:range rdf:resource="#WsdlInputMessageMapList"/>
</owl:ObjectProperty>
<owl:FunctionalProperty rdf:about="#wsdlInputs"/>

<!-- wsdlOutputs -->

<owl:ObjectProperty rdf:ID="wsdlOutputs">
  <rdfs:comment>
    Deprecated as of OWL-S 1.0.  wsdlOutput should be used.
  </rdfs:comment>
  <rdfs:comment>
    A list of WsdlMessageMap instances, one for each
    output of the atomic process.
  </rdfs:comment>
  <rdfs:domain rdf:resource="#WsdlAtomicProcessGrounding"/>
  <rdfs:range rdf:resource="#WsdlOutputMessageMapList"/>
</owl:ObjectProperty>
<owl:FunctionalProperty rdf:about="#wsdlOutputs"/>

<owl:Class rdf:ID="WsdlOutputMessageMapList">
<rdfs:comment> Deprecated as of version 1.1; no longer needed </rdfs:comment>
<rdfs:comment> A list of WsdlOutputMessageMap instances </rdfs:comment>
  <rdfs:subClassOf rdf:resource="&shadow-rdf;#List"/>
  <rdfs:subClassOf>
   <owl:Restriction>
     <owl:onProperty rdf:resource="&shadow-rdf;#first"/>
     <owl:allValuesFrom rdf:resource="#WsdlOutputMessageMap"/>
   </owl:Restriction>
  </rdfs:subClassOf>
  <rdfs:subClassOf>
   <owl:Restriction>
     <owl:onProperty rdf:resource="&shadow-rdf;#rest"/>
     <owl:allValuesFrom rdf:resource="#WsdlOutputMessageMapList"/>
   </owl:Restriction>
  </rdfs:subClassOf>
</owl:Class>

<owl:Class rdf:ID="WsdlInputMessageMapList">
<rdfs:comment> Deprecated as of version 1.1; no longer needed </rdfs:comment>
<rdfs:comment> A list of WsdlInputMessageMap instances </rdfs:comment>
  <rdfs:subClassOf rdf:resource="&shadow-rdf;#List"/>
  <rdfs:subClassOf>
   <owl:Restriction>
     <owl:onProperty rdf:resource="&shadow-rdf;#first"/>
     <owl:allValuesFrom rdf:resource="#WsdlInputMessageMap"/>
   </owl:Restriction>
  </rdfs:subClassOf>
  <rdfs:subClassOf>
   <owl:Restriction>
     <owl:onProperty rdf:resource="&shadow-rdf;#rest"/>
     <owl:allValuesFrom rdf:resource="#WsdlInputMessageMapList"/>
   </owl:Restriction>
  </rdfs:subClassOf>
</owl:Class>

</rdf:RDF>


